binary LR with ref

lean/STLC/STLC/Smallstep_Ref_Equiv.lean
@@ -15,8 +15,7 @@ inductive ty : Type
 | arrow : ty → ty → ty
 
 inductive tm : Type
-| fls : tm
-| tru : tm
+| bool : Bool → tm
 | bvar : ℕ → tm
 | fvar : ℕ → tm
 | abs : tm → tm
@@ -33,7 +32,7 @@ abbrev venv := List tm
 @[simp]
 def openSubst (t1: tm) (n: ℕ) (t2: tm) : tm :=
   match t1 with
-  | .fls | .tru => t1
+  | .bool b => .bool b
   | .bvar x =>
     if x = n then t2
     -- else if n < x then .bvar (x - 1)
@@ -50,7 +49,7 @@ def openSubst (t1: tm) (n: ℕ) (t2: tm) : tm :=
 @[simp]
 def close (t1: tm) (n: ℕ) (m: ℕ) : tm :=
   match t1 with
-  | .fls | .tru => t1
+  | .bool b => .bool b
   | .bvar x => .bvar x
   | .fvar x => if x = n then (.bvar m) else t1
   | .abs t1 => .abs (close t1 n (m + 1))
@@ -64,7 +63,7 @@ def close (t1: tm) (n: ℕ) (m: ℕ) : tm :=
 @[simp]
 def substF (Δ: venv) (t: tm) : tm :=
   match t with
-  | .fls | .tru => t
+  | .bool b => .bool b
   | .bvar _ => t
   | .fvar x =>
     match indexr x Δ with
@@ -80,7 +79,7 @@ def substF (Δ: venv) (t: tm) : tm :=
 @[simp]
 def closedF (t: tm) (n: ℕ) : Prop :=
   match t with
-  | .fls | .tru => true
+  | .bool _ => true
   | .bvar _ => true
   | .fvar x => x < n
   | .abs t1 => closedF t1 n
@@ -93,7 +92,7 @@ def closedF (t: tm) (n: ℕ) : Prop :=
 @[simp]
 def closedB (t: tm) (n: ℕ) : Prop :=
   match t with
-  | .fls | .tru => true
+  | .bool _ => true
   | .bvar x => x < n
   | .fvar _ => true
   | .abs t1 => closedB t1 (n + 1)
@@ -106,7 +105,7 @@ def closedB (t: tm) (n: ℕ) : Prop :=
 @[simp]
 def closedL (t: tm) (n: ℕ) : Prop :=
   match t with
-  | .fls | .tru => true
+  | .bool _ => true
   | .bvar _ => true
   | .fvar _ => true
   | .abs t1 => closedL t1 n
@@ -124,9 +123,9 @@ lemma openClosed : ∀ t n m,
     by_cases hx: (x = m)
     . omega
     . by_cases hx': (x < m)
-      omega; unfold openSubst at h;
-      rw [if_neg hx] at h; have hx'' : (m < x) := by omega;
-      simp [hx''] at h; omega
+      omega; unfold openSubst at h
+      rw [if_neg hx] at h; have hx'' : (m < x) := by omega
+      simp at h; omega
   case abs t ih =>
     apply ih n (m+1); unfold openSubst at h; simp at h; assumption
   case app t1 t2 ih1 ih2 =>
@@ -265,8 +264,7 @@ def binds x τ (Γ : tenv) := (indexr x Γ = some τ)
 abbrev stty := List ty -- Φ, restricted to List .bool
 
 inductive hasType : stty → tenv → tm → ty → Prop
-| fls : ∀ Φ Γ, hasType Φ Γ .fls .bool
-| tru : ∀ Φ Γ, hasType Φ Γ .tru .bool
+| bool : ∀ Φ Γ b, hasType Φ Γ (.bool b) .bool
 | var : ∀ Φ Γ x τ, binds x τ Γ → hasType Φ Γ (.fvar x) τ
 | abs : ∀ Φ Γ t τ₁ τ₂,
   hasType Φ (τ₁::Γ) (openSubst t 0 (.fvar Γ.length)) τ₂ →
@@ -276,23 +274,22 @@ inductive hasType : stty → tenv → tm → ty → Prop
   hasType Φ Γ t₁ (.arrow τ₁ τ₂) →
   hasType Φ Γ t₂ τ₁ →
   hasType Φ Γ (.app t₁ t₂) τ₂
-| loc : ∀ Φ Γ n,
-  n < Φ.length →
-  hasType Φ Γ (.loc n) (.ref .bool)
+--| loc : ∀ Φ Γ n,
+--  n < Φ.length →
+--  hasType Φ Γ (.loc n) (.ref .bool)
 | ref : ∀ Φ Γ t,
   hasType Φ Γ t (.bool) →
   hasType Φ Γ (.ref t) (.ref .bool)
 | deref : ∀ Φ Γ t τ,
-  hasType Φ Γ t (.ref τ) →
-  hasType Φ Γ (.deref t) τ
+  hasType Φ Γ t (.ref .bool) →
+  hasType Φ Γ (.deref t) .bool
 | assign : ∀ Φ Γ t₁ t₂ τ,
-  hasType Φ Γ t₁ (.ref τ) →
-  hasType Φ Γ t₂ τ →
+  hasType Φ Γ t₁ (.ref .bool) →
+  hasType Φ Γ t₂ .bool →
   hasType Φ Γ (.assign t₁ t₂) .bool -- for simplicity, we use bool for the result, could be unit
 
 inductive value : tm → Prop
-| fls : value .fls
-| tru : value .tru
+| bool : ∀ b, value (.bool b)
 | loc : ∀ n, value (.loc n)
 | abs : ∀ t, value (.abs t)
 
@@ -322,7 +319,7 @@ inductive step : st → tm → st → tm → Prop
   step σ t σ' t' →
   step σ (.deref t) σ' (.deref t')
 | assign_val : ∀ σ n v,
-  n < σ.length →
+  -- n < σ.length →
   value v →
   step σ (.assign (.loc n) v) (update σ n v) v
 | assign1 : ∀ σ σ' t1 t1' t2,
@@ -337,6 +334,12 @@ inductive stepn : st → tm → st → tm → Prop
 | refl : ∀ σ t, stepn σ t σ t
 | multi : ∀ σ1 σ2 σ3 t1 t2 t3, stepn σ1 t1 σ2 t2 → step σ2 t2 σ3 t3 → stepn σ1 t1 σ3 t3
 
+lemma stepnTrans : ∀ σ1 σ2 σ3 t1 t2 t3, stepn σ1 t1 σ2 t2 → stepn σ2 t2 σ3 t3 → stepn σ1 t1 σ3 t3 := by
+  intros σ1 σ2 σ3 t1 t2 t3 h1 h2; induction h2
+  . assumption
+  . case _ _ _ _ _ _ hstn hst ih =>
+    apply stepn.multi; apply ih; assumption; assumption
+
 lemma stepnApp1 : ∀ σ1 σ2 t1 t1' t2,
   stepn σ1 t1 σ2 t1' → stepn σ1 (.app t1 t2) σ2 (.app t1' t2) := by
   intros σ1 σ2 t1 t1' t2 h; induction h
@@ -349,6 +352,27 @@ lemma stepnApp2 : ∀ σ1 σ2 t1 t2 t2',
   . constructor
   . case _ hstn hst ih => apply stepn.multi; assumption; apply step.app2; assumption; assumption
 
+lemma stepnBetaVal : ∀ σ1 t v,
+  value v → stepn σ1 (.app (.abs t) v) σ1 (openSubst t 0 v) := by
+  intros σ1 t v hv; apply stepn.multi; apply stepn.refl
+  apply step.beta; assumption
+
+lemma stepnBeta : ∀ σ1 σ2 σ3 σ4 f1 f2 t1 t2 t3,
+  stepn σ1 f1 σ2 (.abs f2) →
+  stepn σ2 t1 σ3 t2 →
+  value t2 →
+  stepn σ3 (openSubst f2 0 t2) σ4 t3 →
+  stepn σ1 (.app f1 t1) σ4 t3 := by
+  intros σ1 σ2 σ3 σ4 f1 f2 t1 t2 t3 h1 h2 hv h3
+  have hstn1: stepn σ1 (.app f1 t1) σ2 (.app (.abs f2) t1) := by apply stepnApp1; assumption
+  have hstn2: stepn σ2 (.app (.abs f2) t1) σ3 (.app (.abs f2) t2) := by apply stepnApp2; constructor; assumption
+  have hstn3: stepn σ3 (.app (.abs f2) t2) σ3 (openSubst f2 0 t2) := by apply stepnBetaVal; assumption
+  have hstn5: stepn σ1 (.app f1 t1) σ4 t3 := by
+    apply stepnTrans; apply hstn1;
+    apply stepnTrans; apply hstn2;
+    apply stepnTrans; apply hstn3; assumption
+  assumption
+
 lemma stepnRef : ∀ σ1 σ2 t1 t2,
   stepn σ1 t1 σ2 t2 → stepn σ1 (.ref t1) σ2 (.ref t2) := by
   intros σ1 σ2 t1 t2 h; induction h
@@ -360,11 +384,45 @@ lemma stepnRefVal : ∀ σ1 v,
   intros σ1 v hv; apply stepn.multi; apply stepn.refl;
   apply step.ref_val; assumption
 
-lemma stepnTrans : ∀ σ1 σ2 σ3 t1 t2 t3, stepn σ1 t1 σ2 t2 → stepn σ2 t2 σ3 t3 → stepn σ1 t1 σ3 t3 := by
-  intros σ1 σ2 σ3 t1 t2 t3 h1 h2; induction h2
-  . assumption
-  . case _ _ _ _ _ _ hstn hst ih =>
-    apply stepn.multi; apply ih; assumption; assumption
+lemma stepnDeref : ∀ σ1 σ2 t1 t2,
+  stepn σ1 t1 σ2 t2 → stepn σ1 (.deref t1) σ2 (.deref t2) := by
+  intros σ1 σ2 t1 t2 h; induction h
+  . constructor
+  . case _ hstn hst ih => constructor; assumption; apply step.deref; assumption
+
+lemma stepnDerefVal : ∀ σ l v,
+  indexr l σ = some v → stepn σ (.deref (.loc l)) σ v := by
+  intros σ l v h; apply stepn.multi; apply stepn.refl;
+  apply step.deref_val; assumption
+
+lemma stepnAssign1 : ∀ σ1 σ2 t1 t1' t2,
+  stepn σ1 t1 σ2 t1' → stepn σ1 (.assign t1 t2) σ2 (.assign t1' t2) := by
+  intros σ1 σ2 t1 t1' t2 h; induction h
+  . constructor
+  . case _ hstn hst ih => constructor; assumption; apply step.assign1; assumption
+
+lemma stepnAssign2: ∀ σ1 σ2 t1 t2 t2',
+  value t1 → stepn σ1 t2 σ2 t2' → stepn σ1 (.assign t1 t2) σ2 (.assign t1 t2') := by
+  intros σ1 σ2 t1 t2 t2' hv h; induction h
+  . constructor
+  . case _ hstn hst ih => apply stepn.multi; assumption; apply step.assign2; assumption; assumption
+
+lemma stepnAssignVal : ∀ σ1 n v,
+  value v → stepn σ1 (.assign (.loc n) v) (update σ1 n v) v := by
+  intros σ1 n v hv; apply stepn.multi; apply stepn.refl;
+  apply step.assign_val; assumption
+
+lemma stepnAssign : ∀ σ1 σ2 σ3 t1 t2 l v,
+  stepn σ1 t1 σ2 (tm.loc l) →
+  stepn σ2 t2 σ3 v →
+  value v →
+  stepn σ1 (.assign t1 t2) (update σ3 l v) v := by
+  intros σ1 σ2 σ3 t1 t2 l v h1 h2 hv;
+  have hstn1: stepn σ1 (.assign t1 t2) σ2 (.assign (.loc l) t2) := by apply stepnAssign1; assumption
+  have hstn2: stepn σ2 (.assign (.loc l) t2) σ3 (.assign (.loc l) v) := by apply stepnAssign2; constructor; assumption
+  have hstn3: stepn σ1 (.assign t1 t2) σ3 (.assign (.loc l) v) := by apply stepnTrans <;> assumption
+  have hstn4: stepn σ3 (.assign (.loc l) v) (update σ3 l v) v := by apply stepnAssignVal; assumption
+  apply stepnTrans; apply hstn3; apply hstn4
 
 -- the "world"
 @[simp]
@@ -389,13 +447,12 @@ def bijection {X Y} (f: X → Y → Prop): Prop :=
 
 @[simp]
 def storeType (σ1 σ2 : st) (m : st_rel) : Prop :=
-  (∀ l1 l2, m l1 l2 → ∃ v, indexr l1 σ1 = some v ∧ indexr l2 σ2 = some v) ∧ bijection m
+  (∀ l1 l2, m l1 l2 → ∃ v, indexr l1 σ1 = some (.bool v) ∧ indexr l2 σ2 = some (.bool v)) ∧ bijection m
 
 @[simp]
 def valType (m: st_rel) (t1 : tm) (t2 : tm) (τ : ty) : Prop :=
   match t1, t2, τ with
-  | .fls, .fls, .bool => true
-  | .tru, .tru, .bool => true
+  | .bool b1, .bool b2, .bool => b1 = b2
   | .loc n1, .loc n2, .ref τ => m n1 n2
   | (.abs t1), (.abs t2), .arrow τ1 τ2 =>
     ∀ v1 v2 m1 st1 st2,
@@ -403,8 +460,8 @@ def valType (m: st_rel) (t1 : tm) (t2 : tm) (τ : ty) : Prop :=
     storeType st1 st2 m1 →
     valType m1 v1 v2 τ1 → closedB v1 0 → closedB v2 0 →
     ∃ v3 v4 m2 st1' st2',
-    m1 ≥ m2 →
-    storeType st1' st2' m2 →
+    m1 ≥ m2 ∧
+    storeType st1' st2' m2 ∧
     stepn st1 (openSubst t1 0 v1) st1' v3 ∧ closedB v3 0 ∧
     stepn st2 (openSubst t2 0 v2) st2' v4 ∧ closedB v4 0 ∧
     valType m2 v3 v4 τ2
@@ -443,10 +500,7 @@ def semType (Γ : tenv) (t1 t2 : tm) (τ : ty) : Prop :=
 
 lemma valTypeValue : ∀ m t1 t2 τ, valType m t1 t2 τ → value t1 ∧ value t2 := by
   intros m t1 t2 τ h; cases t1 <;> cases t2 <;> try simp at h
-  . apply And.intro <;> constructor
-  . apply And.intro <;> constructor
-  . next t1 t2 => apply And.intro <;> apply value.abs
-  . apply And.intro <;> constructor
+  repeat apply And.intro <;> constructor
 
 lemma extend.refl : ∀ m, m ≥ m := by intros m a b h; assumption
 
@@ -457,8 +511,8 @@ lemma extend.ext : ∀ st1 st2 m,
   intros st1 st2 m h; simp;
   intros a b h'; right; rcases h with ⟨h1, h2⟩;
   specialize h1 _ _ h'; rcases h1 with ⟨v, hidx1, hidx2⟩;
-  apply And.intro; apply indexrSome'' _ _ ⟨v, hidx1⟩
-  apply And.intro; apply indexrSome'' _ _ ⟨v, hidx2⟩
+  apply And.intro; apply indexrSome'' _ _ ⟨.bool v, hidx1⟩
+  apply And.intro; apply indexrSome'' _ _ ⟨.bool v, hidx2⟩
   assumption
 
 lemma extend.trans : ∀ {m1 m2 m3},
@@ -516,10 +570,9 @@ lemma storeType.ext : ∀ σ1 σ2 m v1 v2,
   apply And.intro
   . intros l1 l2 m'; cases m' with
     | inl h =>
-      rcases h with ⟨hidx1, hidx2⟩
-      rw [hidx1, hidx2]; rw [indexrHead]; rw [indexrHead]
+      rw [h.1, h.2]; rw [indexrHead]; rw [indexrHead]
       cases v1 <;> cases v2 <;> simp at hv12
-      exists .fls; exists .tru
+      rename_i v1 v2; rw [hv12]; exists v2
     | inr h =>
       specialize h1 l1 l2 h.2.2
       rcases h1 with ⟨v, hidx1, hidx2⟩
@@ -530,32 +583,33 @@ lemma storeType.update : ∀ st1 st2 m v1 v2 l1 l2,
   storeType st1 st2 m →
   valType m v1 v2 .bool →
   m l1 l2 →
-  storeType (update st1 l1 v1) (update st2 l2 v2) (st_rel.ext m l1 l2) := by
+  storeType (update st1 l1 v1) (update st2 l2 v2) m := by
   intros st1 st2 m v1 v2 l1 l2 hst hv12 hm
-  rcases hst with ⟨h1, h2⟩
+  rcases hst with ⟨h1, h2, h3⟩
   apply And.intro
-  . intros l1' l2' m'
-    by_cases h': l1 = l1' <;> by_cases h'': l2 = l2' <;> simp [h', h''] at m' <;> try omega
+  . intros l1' l2' hm'
+    by_cases h': l1 = l1' <;> by_cases h'': l2 = l2'
     . subst h'; subst h''
       specialize h1 l1 l2 hm; rcases h1 with ⟨v, hidx1, hidx2⟩
       rw [indexrUpdateHit]; rw [indexrUpdateHit]
-      cases v1 <;> cases v2 <;> simp at hv12; exists .fls; exists .tru
-      apply indexrSome'; exists v; apply indexrSome'; exists v
-    . cases m' with
-      | inl h => aesop
-      | inr h =>
-        specialize h1 l1' l2' h.2.2
-        rcases h1 with ⟨v, hidx1, hidx2⟩
-        exists v; rw [indexrUpdateMiss]; rw [indexrUpdateMiss];
-        apply And.intro <;> assumption; omega; omega
-  . rcases h2 with ⟨h21, h22⟩; aesop
+      cases v1 <;> cases v2 <;> simp at hv12;
+      rename_i v1 v2; rw [hv12]; exists v2
+      apply indexrSome'; grind; apply indexrSome'; grind
+    . subst h'; have c : l2 = l2' := by apply h2; apply hm; apply hm'
+      contradiction
+    . subst h''; have c : l1 = l1' := by apply h3; apply hm; apply hm'
+      contradiction
+    . specialize h1 l1' l2' hm'; rcases h1 with ⟨v, hidx1, hidx2⟩
+      exists v; rw [indexrUpdateMiss]; rw [indexrUpdateMiss];
+      apply And.intro <;> assumption; omega; omega
+  . aesop
 
 lemma valType.antimono : ∀ m1 m2 v1 v2 τ,
   valType m1 v1 v2 τ → m1 ≥ m2 → valType m2 v1 v2 τ := by
   intros m1 m2 v1 v2 τ hv12 hm;
   cases v1 <;> cases v2 <;> try simp at hv12
-  . cases τ <;> try simp at hv12 <;> simp
-  . cases τ <;> try simp at hv12 <;> simp
+  . rename_i v1 v2;
+    cases v1 <;> cases v2 <;> cases τ <;> try simp at hv12 <;> simp
   . cases τ; simp at hv12; simp at hv12
     next t1 t2 τ1 τ2 =>
     intros v3 v4 m3 st1 st2 hm'
@@ -571,15 +625,9 @@ lemma envType.antimono : ∀ m1 m2 Δ1 Δ2 Γ,
 
 -- compatibility lemmas
 
-lemma semTrue : ∀ Γ, semType Γ .tru .tru .bool := by
-  intros Γ st1 st2 m Δ1 Δ2 _ _ _ _;
-  exists st1, st2, m, .tru, .tru;
-  apply And.intro; apply extend.refl; apply And.intro; assumption;
-  simp; apply And.intro <;> apply stepn.refl
-
-lemma semFalse : ∀ Γ, semType Γ .fls .fls .bool := by
-  intros Γ st1 st2 m Δ1 Δ2 _ _ _ _;
-  exists st1, st2, m, .fls, .fls;
+lemma semBool : ∀ Γ b, semType Γ (.bool b) (.bool b) .bool := by
+  intros Γ b st1 st2 m Δ1 Δ2 _ _ _ _;
+  exists st1, st2, m, (.bool b), (.bool b);
   apply And.intro; apply extend.refl; apply And.intro; assumption;
   simp; apply And.intro <;> apply stepn.refl
 
@@ -588,7 +636,7 @@ lemma semVar : ∀ Γ x τ, binds x τ Γ → semType Γ (.fvar x) (.fvar x) τ 
   rcases henv with ⟨_, _, h⟩
   have ⟨v1, v2, idx1, cl1, idx2, cl2, semv⟩ := h τ x hbd
   exists st1, st2, m, v1, v2; simp [idx1, idx2]
-  apply And.intro; apply hst
+  apply And.intro; simp at hst; exact hst
   exact ⟨stepn.refl st1 v1, stepn.refl st2 v2, cl1, cl2, semv⟩
 
 lemma semRef : ∀ Γ t1 t2,
@@ -597,10 +645,8 @@ lemma semRef : ∀ Γ t1 t2,
   intros Γ t1 t2 hsem st1 st2 m Δ1 Δ2 wf1 wf2 henv hst
   have hexp := hsem st1 st2 m Δ1 Δ2 wf1 wf2 henv hst
   rcases hexp with ⟨st1', st2', m', v1, v2, hm1, hstore, hstep1, hstep2, hcl1, hcl2, hv12⟩
-  have hm2 := extend.ext st1' st2' m' hstore
-  have hm3 := extend.trans hm1 hm2
-  exists (v1::st1'), (v2::st2'), (st_rel.ext m' st1'.length st2'.length),
-         (.loc st1'.length), (.loc st2'.length);
+  have hm3 := extend.trans hm1 (extend.ext st1' st2' m' hstore)
+  exists (v1::st1'), (v2::st2'), (st_rel.ext m' st1'.length st2'.length), (.loc st1'.length), (.loc st2'.length)
   constructor; apply hm3
   constructor; apply storeType.ext; assumption; assumption
   simp; constructor; apply stepnTrans; apply stepnRef; apply hstep1
@@ -610,14 +656,196 @@ lemma semRef : ∀ Γ t1 t2,
 
 lemma semDeref : ∀ Γ t1 t2,
   semType Γ t1 t2 (.ref .bool) →
-  semType Γ (.deref t1) (.deref t2) .bool := by sorry
+  semType Γ (.deref t1) (.deref t2) .bool := by
+  intros Γ t1 t2 hsem st1 st2 m Δ1 Δ2 wf1 wf2 henv hst
+  have hexp := hsem st1 st2 m Δ1 Δ2 wf1 wf2 henv hst
+  rcases hexp with ⟨st1', st2', m', v1, v2, hm1, hstore, hstep1, hstep2, hv12⟩
+  cases v1 <;> cases v2 <;> simp at hv12
+  rename_i l1 l2; rcases hstore.1 l1 l2 hv12 with ⟨b, hidx1, hidx2⟩
+  exists st1', st2', m', .bool b, .bool b;
+  apply And.intro; assumption; apply And.intro; assumption; simp
+  apply And.intro
+  . have hstn1 : stepn st1 (.deref (substF Δ1 t1)) st1' (.deref (.loc l1)) := by
+      apply stepnDeref; assumption
+    have hstn2 : stepn st1' (.deref (.loc l1)) st1' (.bool b) := by
+      apply stepnDerefVal; assumption
+    apply stepnTrans; apply hstn1; apply hstn2
+  . have hstn1 : stepn st2 (.deref (substF Δ2 t2)) st2' (.deref (.loc l2)) := by
+      apply stepnDeref; assumption
+    have hstn2 : stepn st2' (.deref (.loc l2)) st2' (.bool b) := by
+      apply stepnDerefVal; assumption
+    apply stepnTrans; apply hstn1; apply hstn2
+
+lemma wfAssign : ∀ {t1 t2 Γ},
+  wf (.assign t1 t2) Γ →  wf t1 Γ ∧ wf t2 Γ := by
+  intros t1 t2 Γ h; simp at h; constructor; aesop; aesop
+
+lemma wfApp : ∀ {f t Γ},
+  wf (.app f t) Γ →  wf f Γ ∧ wf t Γ := by
+  intros f t Γ h; simp at h; constructor; aesop; aesop
 
 lemma semAssign : ∀ Γ t1 t2 t1' t2',
   semType Γ t1 t1' (.ref .bool) →
   semType Γ t2 t2' .bool →
-  semType Γ (.assign t1 t2) (.assign t1' t2') .bool := by sorry
+  semType Γ (.assign t1 t2) (.assign t1' t2') .bool := by
+  intros Γ t1 t2 t1' t2' hsem1 hsem2 st1 st2 m Δ1 Δ2 wf1 wf2 henv hst
+  have hexp1 := hsem1 st1 st2 m Δ1 Δ2 (wfAssign wf1).1 (wfAssign wf2).1 henv hst
+  rcases hexp1 with ⟨st1', st2', m', v1, v2, hm1, hstore, hstep1, hstep2, hclv1, hclv2, hv12⟩
+  have henv' : envType m' Δ1 Δ2 Γ := by apply envType.antimono; apply henv; apply hm1
+  have hexp2 := hsem2 st1' st2' m' Δ1 Δ2 (wfAssign wf1).2 (wfAssign wf2).2 henv' hstore
+  rcases hexp2 with ⟨st1'', st2'', m'', v1', v2', hm2, hstore2, hstep1', hstep2', hclv1', hclv2', hv12'⟩
+  cases v1 <;> cases v2 <;> simp at hv12
+  rename_i l1 l2; rcases hstore.1 l1 l2 hv12 with ⟨b, hidx1, hidx2⟩
+  exists (update st1'' l1 v1'), (update st2'' l2 v2'), m'', v1', v2'
+  constructor; apply extend.trans; apply hm1; apply hm2
+  constructor; apply storeType.update; assumption; assumption; apply hm2; assumption
+  apply And.intro
+  . simp; have hv := (valTypeValue _ _ _ _ hv12').1
+    apply stepnAssign <;> assumption
+  . constructor; have hv := (valTypeValue _ _ _ _ hv12').2
+    apply stepnAssign <;> assumption; grind
 
 lemma semApp : ∀ Γ f1 f2 t1 t2 τ1 τ2,
   semType Γ f1 f2 (.arrow τ1 τ2) →
   semType Γ t1 t2 τ1 →
-  semType Γ (.app f1 t1) (.app f2 t2) τ2 := by sorry
+  semType Γ (.app f1 t1) (.app f2 t2) τ2 := by
+  intros Γ f1 f2 t1 t2 τ1 τ2 hsemf hsemt st1 st2 m Δ1 Δ2 wf1 wf2 henv hst
+  have hexpf := hsemf st1 st2 m Δ1 Δ2 (wfApp wf1).1 (wfApp wf2).1 henv hst
+  rcases hexpf with ⟨st1', st2', m1, f1', f2', hm1, hstore, hstepf1, hstepf2, hclf1, hclf2, hf12⟩
+  have henv' : envType m1 Δ1 Δ2 Γ := by apply envType.antimono; apply henv; apply hm1
+  have hexpt := hsemt st1' st2' m1 Δ1 Δ2 (wfApp wf1).2 (wfApp wf2).2 henv' hstore
+  rcases hexpt with ⟨st1'', st2'', m2, t1', t2', hm2, hstore2, hstept1, hstept2, hclt1, hclt2, ht12⟩
+  cases f1' <;> cases f2' <;> try contradiction
+  rename_i t3 t4
+  specialize hf12 t1' t2' m2 st1'' st2'' hm2 hstore2 ht12 hclt1 hclt2
+  have ⟨v5, v6, m3, st3, st4, hm3, hstore3, hstbt1, hstbt2, hclv5, hclv6, hv56⟩ := hf12
+  exists st3, st4, m3, v5, v6
+  constructor; apply extend.trans; apply hm1; apply extend.trans; apply hm2; apply hm3
+  constructor; assumption; constructor; simp
+  apply stepnBeta; assumption; assumption; exact (valTypeValue _ _ _ _ ht12).1
+  assumption; constructor; simp
+  apply stepnBeta; assumption; assumption; exact (valTypeValue _ _ _ _ ht12).2
+  assumption; constructor; assumption; constructor; assumption; assumption
+
+lemma lenInc: ∀ {A} x (L : List A), L.length + 1 = (x::L).length := by intros _ L x; simp
+
+lemma envTypeClosed : ∀ m Δ1 Δ2 Γ, envType m Δ1 Δ2 Γ →
+  (∀ x t1, indexr x Δ1 = some t1 → closedB t1 0) ∧
+  (∀ x t1, indexr x Δ2 = some t1 → closedB t1 0) := by
+  intros m Δ1 Δ2 Γ henv; rcases henv with ⟨hlen1, hlen2, h⟩
+  apply And.intro
+  . intros x t1 hidx;
+    have hx : (x < Δ1.length) := by apply indexrSome'; exists t1
+    rw [hlen1] at hx; have hidx' := indexrSome Γ x hx
+    rcases hidx' with ⟨τ, hidx'⟩;
+    have ⟨v1, v2, hidxv1, hclv1, hidxv2, hclv2, hval⟩  := h τ x hidx'
+    rw [hidx] at hidxv1; cases hidxv1; assumption
+  . intros x t1 hidx;
+    have hx : (x < Δ2.length) := by apply indexrSome'; exists t1
+    rw [hlen2] at hx; have hidx' := indexrSome Γ x hx
+    rcases hidx' with ⟨τ, hidx'⟩;
+    have ⟨v1, v2, hidxv1, hclv1, hidxv2, hclv2, hval⟩  := h τ x hidx'
+    rw [hidx] at hidxv2; cases hidxv2; assumption
+
+lemma envTypeExtend : ∀ m Δ1 Δ2 Γ v1 v2 τ,
+  envType m Δ1 Δ2 Γ →
+  closedB v1 0 → closedB v2 0 →
+  valType m v1 v2 τ →
+  envType m (v1::Δ1) (v2::Δ2) (τ::Γ) := by
+  intros m Δ1 Δ2 Γ v1 v2 τ henv hclv1 hclv2 hv12
+  constructor; simp; apply henv.1
+  constructor; simp; apply henv.2.1
+  intros τ' x hbd; rcases henv with ⟨hlen1, hlen2, h⟩
+  by_cases hx: (x = Δ1.length)
+  . simp [hx]; constructor; assumption; simp [hlen1, hlen2]
+    constructor; assumption; simp at hbd; simp [hx, hlen1] at hbd
+    rw [<- hbd]; assumption
+  . simp at hbd; rw [<-hlen1, if_neg hx] at hbd;
+    simp; rw [if_neg hx]; rw [hlen2, <-hlen1, if_neg hx]
+    specialize h τ' x hbd; rcases h with ⟨v1, v2, h⟩
+    exists v1; constructor; exact h.1; constructor; exact h.2.1
+    exists v2; exact h.2.2
+
+lemma semAbs : ∀ Γ t1 t2 τ1 τ2,
+  semType (τ1::Γ) (openSubst t1 0 (.fvar Γ.length)) (openSubst t2 0 (.fvar Γ.length)) τ2 →
+  semType Γ (.abs t1) (.abs t2) (.arrow τ1 τ2) := by
+  intros Γ t1 t2 τ1 τ2 hsem st1 st2 m Δ1 Δ2 wf1 wf2 henv hst
+  exists st1, st2, m, (substF Δ1 (.abs t1)), (substF Δ2 (.abs t2))
+  constructor; apply extend.refl; constructor; assumption
+  constructor; apply stepn.refl
+  constructor; apply stepn.refl
+  simp at wf1; simp at wf2
+  have hclb1' := openClosed' t1 (Γ.length) 0 wf1.1
+  have hclb2' := openClosed' t2 (Γ.length) 0 wf2.1
+  have envcl := envTypeClosed m Δ1 Δ2 Γ henv
+  constructor; apply substFClosedBComm _ _ _ envcl.1 wf1.1
+  constructor; apply substFClosedBComm _ _ _ envcl.2 wf2.1
+  intros v1 v2 m' st1' st2' hm hst hval12 hclv1 hclv2
+  have henv1 := envType.antimono m m' Δ1 Δ2 Γ henv hm
+  have henv2 := envTypeExtend m' Δ1 Δ2 Γ v1 v2 τ1 henv1 hclv1 hclv2 hval12
+  have clf1' := closedFInc _ _ 0 wf1.2
+  have clf2' := closedFInc _ _ 0 wf2.2
+  have hsem' := hsem st1' st2' m' (v1::Δ1) (v2::Δ2) ⟨hclb1', clf1'⟩ ⟨hclb2', clf2'⟩ henv2 hst
+  rcases hsem' with ⟨st1'', st2'', m'', vr1, vr2, hm', hst'', hst1, hst2, hclvr1, hclvr2, semvr⟩
+  rw [<-henv.1] at hst1; rw [<-henv.2.1] at hst2
+  rw [substFOpenComm] at hst1; rw [substFOpenComm] at hst2
+  exists vr1, vr2, m'', st1'', st2''
+  rw [henv.2.1]; exact wf2.2;  exact envcl.2; rw [henv.1]; exact wf1.2; exact envcl.1
+
+theorem fundamental : ∀ Φ Γ t τ,
+  hasType Φ Γ t τ → semType Γ t t τ := by
+  intros Φ Γ t τ h; induction h
+  case bool => apply semBool
+  case var => apply semVar; assumption
+  case abs => apply semAbs; assumption
+  case app => apply semApp <;> assumption
+  case ref => apply semRef; assumption
+  case deref => apply semDeref; assumption
+  case assign => apply semAssign <;> assumption
+
+lemma hasTypeClosedB : ∀ Φ Γ t τ, hasType Φ Γ t τ → closedB t 0 := by
+  intros Φ Γ t τ h; induction h <;> simp
+  case abs => apply openClosed; assumption
+  case app => apply And.intro <;> assumption
+  case ref => assumption
+  case deref => assumption
+  case assign => apply And.intro <;> assumption
+
+lemma substFMt: ∀ t, substF [] t = t := by
+  intros t; induction t <;> simp <;> try assumption
+  apply And.intro <;> assumption
+  apply And.intro <;> assumption
+
+lemma hasTypeClosedF : ∀ Φ t τ, hasType Φ [] t τ → closedF t 0 := by
+  intros Φ t τ h; revert τ; induction t <;> intros τ h <;> simp
+  . case fvar x => cases h; next bd => simp at bd
+  . case abs t ih => cases h; assumption
+  . case app t1 t2 ih1 ih2 =>
+    cases h; apply And.intro
+    . apply ih1; assumption
+    . apply ih2; assumption
+  . case ref t ih => cases h; apply ih; assumption
+  . case deref t ih => cases h; apply ih; assumption
+  . case assign t1 t2 ih1 ih2 =>
+    cases h; apply And.intro
+    . apply ih1; assumption
+    . apply ih2; assumption
+
+lemma hasTypeWf : ∀ Φ t τ, hasType Φ [] t τ → wf t [] := by
+  intros Φ t τ h; constructor
+  . apply hasTypeClosedB; assumption
+  . apply hasTypeClosedF; assumption
+
+theorem safety : ∀ t τ, hasType [] [] t τ → expType [] [] st_rel.mt t t τ := by
+  intros t τ h
+  have hsem := fundamental [] [] t τ h
+  have henv : envType st_rel.mt [] [] [] := by apply envType.empty
+  have hst : storeType [] [] st_rel.mt := by apply storeType.mt
+  have hexp := hsem [] [] st_rel.mt [] [] (hasTypeWf [] t τ h) (hasTypeWf [] t τ h) henv hst
+  rcases hexp with ⟨st1, st2, m, v1, v2, hm, hstore, hst1, hst2, hclb1, hclb2, hval⟩
+  exists st1, st2, m, v1, v2
+  constructor; assumption
+  constructor; assumption
+  constructor; rw [substFMt] at hst1; assumption
+  constructor; rw [substFMt] at hst2; assumption
+  exact ⟨hclb1, hclb2, hval⟩
